nola/examples/logic/iris.v
@@ -10,8 +10,8 @@ From nola.examples.heap_lang Require Export definitions.
 (** [nintpGS]: Iris resource *)
 Class nintpGS Σ := NintpGS {
   nintpGS_sinv :: sinvGS (nPropSO (;ᵞ)) Σ;
-  nintpGS_ninv :: ninvGS (nPropS (;ᵞ)) Σ;
-  nintpGS_na_ninv :: na_ninvGS (nPropS (;ᵞ)) Σ;
+  nintpGS_ninv :: ninvGS (nPropSO (;ᵞ)) Σ;
+  nintpGS_na_ninv :: na_ninvGS (nPropSO (;ᵞ)) Σ;
   nintpGS_na_inv :: na_invG Σ;
   nintpGS_cinv :: cinvG Σ;
   nintpGS_pborrow :: pborrowGS nsynty (nPropS (;ᵞ)) Σ;
