nola/examples/type/rules/conv.v
@@ -115,14 +115,16 @@ Section conv.
     inv_tok tguardN (tinvd_guard T v) -∗ tguard δ (i:=i) T v.
   Proof.
     iIntros "#inv !>". iApply (Deriv_intro (δ:=δ))=>/=. iIntros (?????).
-    iMod (inv_tok_acc with "inv") as "/=[#T cl]"; [done|]. by iMod ("cl" with "T").
+    iMod (inv_tok_acc (intp:=λ _, _) with "inv") as "/=[#T cl]"; [done|].
+    by iMod ("cl" with "T").
   Qed.
   Lemma ttrans_guard_intro `{!tDeriv ih δ, ! i <ⁿ j} {k T} :
     T ==>{_,k}(j,δ) ▽{i,nil} T.
   Proof.
     iIntros (???) "/= #?". iApply fupdw_tinv_wsat_le. iIntros (?).
     have ? : i <ⁿ L by apply (nlt_nle_trans _ _).
-    iMod (inv_tok_alloc (tinvd_guard T _) with "[]") as "inv"; [done|].
+    iMod (inv_tok_alloc (PROP:=tinvdO _) (tinvd_guard T _) with "[]") as "inv";
+      [done|].
     iApply (ninv_tguard with "inv").
   Qed.
 
